Progress

TestModels/Streaming/src/SimpleStreamingImpl.dfy
@@ -2,27 +2,64 @@
 
 
 module Foo {
+
+  // IN STDLIB
+
   trait Action<T, R> {
+    ghost var history: seq<(T, R)>
+
+    ghost predicate Consumes(history: seq<(T, R)>, next: T)
+    ghost predicate Produces(history: seq<(T, R)>)
+    
+
     method Call(t: T) returns (r: R)
+      requires Consumes(history, t)
+
+  }
+
+  type SingleUseAction<T, R> = a: Action<T, R>
+    // TODO: Needs indirection or (!new)
+    // | forall history | a.Produces(history) :: |history| <= 1
+    | true 
+    witness *
+
+  ghost predicate ConsumesAnything<T(!new), R(!new)>(a: Action<T, R>) {
+    forall history, next | a.Produces(history) :: a.Consumes(history, next)
   }
 
   type byte = b: nat | b < 256
   type bytes = seq<byte>
 
-  datatype StreamingBlobInputRequest = StreamingBlobInputRequest()
-  datatype StreamingBlobInputResponse = StreamingBlobInputResponse()
+  datatype StreamingBlobRequest = StreamingBlobRequest()
+  datatype StreamingBlobResponse = StreamingBlobResponse()
+
+  type Error
+
+  datatype Option<T> = Some(value: T) | None
+  datatype Result<T, E> = Success(value: T) | Failure(error: E)
+
+  // GENERATED
 
   // TODO: Check Smithy spec about when response is received
 
-  method StreamingBlobInput(input: StreamingBlobInputRequest, sink: Action<StreamingBlobInputResponse, ()>) 
-    returns (onData: Action<bytes, ()>)
+  // TODO: Spec on when sink will be called vs. onData
+  method StreamingBlobInput(input: StreamingBlobRequest, onResult: SingleUseAction<Result<StreamingBlobResponse, Error>, ()>) 
+    returns (onInputData: Action<Option<bytes>, ()>)
+    // TODO: Should be tightened up to reject any data after None
+    ensures ConsumesAnything(onInputData)
 
+  datatype StreamingBlobOutputEvent =
+    | StreamingBlobOutputData(data: bytes)
+    | StreamingBlobOutputSuccess(response: StreamingBlobResponse)
+    | StreamingBlobOutputFailure(error: Error)
 
-  method StreamingBlobOutput(input: StreamingBlobInputRequest, sink: Action<bytes, ()>) 
-    returns (response: StreamingBlobInputResponse)
+  method StreamingBlobOutput(input: StreamingBlobRequest, onResultEvent: Action<StreamingBlobOutputEvent, ()>) 
+    // TODO: needs a requires clause about sequences of events the callback will consume
 
-
-  method StreamingBlobInputAndOutput(input: StreamingBlobInputRequest, sink: Action<bytes, ()>) 
-    returns (response: StreamingBlobInputResponse, onData: Action<bytes, ()>)
+  method StreamingBlobInputAndOutput(input: StreamingBlobRequest, onResultEvent: Action<StreamingBlobOutputEvent, ()>) 
+    returns (onInputData: Action<Option<bytes>, ()>)
+    // TODO: Should be tightened up to reject any data after None
+    ensures ConsumesAnything(onInputData)
+    // TODO: needs a requires clause about sequences of events the callback will consume
 }
 
